Use modules, simp, grind in chase derivations

ExistentialRules/ChaseSequence/ChaseDerivation.lean
@@ -1,7 +1,9 @@
+module
+
 import BasicLeanDatastructures.Nat
 
-import ExistentialRules.Models.Basic
-import ExistentialRules.ChaseSequence.ChaseDerivationSkeleton
+public import ExistentialRules.Models.Basic
+public import ExistentialRules.ChaseSequence.ChaseDerivationSkeleton
 
 /-!
 # Chase Derivation
@@ -34,7 +36,7 @@ Expressing the conditions in terms of the machinery available form the `Possibly
 As part of the framework built around the `ChaseDerivation`, we will also restate these conditions in a more accessible way. See e.g. `ChaseDerivation.fairness'`.
 -/
 
-structure ChaseDerivation (obs : ObsoletenessCondition sig) (rules : RuleSet sig) extends ChaseDerivationSkeleton obs rules where
+public structure ChaseDerivation (obs : ObsoletenessCondition sig) (rules : RuleSet sig) extends ChaseDerivationSkeleton obs rules where
   triggers_active : ∀ n : Nat, ∀ before ∈ (branch.drop n).head,
     ∀ after ∈ (branch.drop n).tail.head, ∃ orig ∈ after.origin, orig.fst.val.active before.facts
   fairness : ∀ trg : (RTrigger obs rules), ∃ i : Nat, (∃ node ∈ (branch.drop i).head, ¬ trg.val.active node.facts)
@@ -44,7 +46,7 @@ namespace ChaseDerivation
 
 variable {obs : ObsoletenessCondition sig} {rules : RuleSet sig}
 
-section Basics
+public section Basics
 
 /-!
 ## Basic Definitions
@@ -56,7 +58,11 @@ Here we introduce some auxiliary definitions and theorems and we lift some of th
 instance : Membership (ChaseNode obs rules) (ChaseDerivation obs rules) where
   mem cd node := node ∈ cd.toChaseDerivationSkeleton
 
+/-- An element is a member of the derivation iff it occurs at some index in the underlying branch. -/
+theorem mem_iff {cd : ChaseDerivation obs rules} : ∀ {e}, e ∈ cd ↔ ∃ n, cd.branch.get? n = some e := ChaseDerivationSkeleton.mem_iff
+
 /-- Each suffix of the underlying `ChaseDerivationSkeleton` is itself a `ChaseDerivation`. -/
+@[expose]
 def derivation_for_skeleton
     (cd : ChaseDerivation obs rules)
     (l2 : ChaseDerivationSkeleton obs rules)
@@ -66,17 +72,17 @@ def derivation_for_skeleton
   isSome_head := l2.isSome_head
   triggers_exist := l2.triggers_exist
   triggers_active := by
-    rw [ChaseDerivationSkeleton.IsSuffix, PossiblyInfiniteList.IsSuffix_iff] at suffix
+    rw [ChaseDerivationSkeleton.IsSuffix_iff] at suffix
     rcases suffix with ⟨m, suffix⟩
     rw [← suffix]
     intro n
     have := cd.triggers_active (m + n)
-    simp only [PossiblyInfiniteList.head_drop, PossiblyInfiniteList.get?_drop] at *
+    simp only [PossiblyInfiniteList.head_drop, PossiblyInfiniteList.get?_drop, PossiblyInfiniteList.tail_drop] at *
     exact this
   fairness := by
     have l2_head_some := l2.isSome_head
     rw [Option.isSome_iff_exists] at l2_head_some; rcases l2_head_some with ⟨l2_head, l2_head_eq⟩
-    rw [ChaseDerivationSkeleton.IsSuffix, PossiblyInfiniteList.IsSuffix_iff] at suffix
+    rw [ChaseDerivationSkeleton.IsSuffix_iff] at suffix
     rcases suffix with ⟨m, suffix⟩
     rw [← suffix]
     intro trg
@@ -88,10 +94,9 @@ def derivation_for_skeleton
       constructor
       . exists l2_head
         constructor
-        . simp only [PossiblyInfiniteList.drop_zero]; rw [suffix, l2_head_eq]; rfl
+        . grind
         . apply (fairness.right diff)
-          rw [PossiblyInfiniteList.get?_tail, PossiblyInfiniteList.get?_drop, ← PossiblyInfiniteList.head_drop, Nat.succ_eq_add_one, ← Nat.add_assoc, ← lt]
-          rw [suffix, l2_head_eq]; rfl
+          grind
       . intro j
         have fairness := fairness.right (diff.succ + j)
         simp only [PossiblyInfiniteList.drop_zero, PossiblyInfiniteList.get?_tail, PossiblyInfiniteList.get?_drop] at *
@@ -114,9 +119,10 @@ Compared to the `ChaseDerivationSkeleton` we can show some additional results fo
 -/
 
 /-- The trigger used to derive `next` is active for `head`. -/
+@[grind ->]
 theorem active_trigger_origin_next {cd : ChaseDerivation obs rules} {next : ChaseNode obs rules} (eq : cd.next = some next) :
     (next.origin.get (cd.isSome_origin_next eq)).fst.val.active cd.head.facts := by
-  have trg_act := cd.triggers_active 0 cd.head (by simp [PossiblyInfiniteList.drop_zero, ChaseDerivationSkeleton.head]) next eq
+  have trg_act := cd.triggers_active 0 cd.head (by simp [ChaseDerivationSkeleton.head]) next (by simp [← eq, ChaseDerivationSkeleton.next])
   rcases trg_act with ⟨orig, orig_mem, trg_act⟩
   rw [Option.mem_def] at orig_mem
   simp only [orig_mem, Option.get_some]
@@ -138,12 +144,12 @@ theorem isSome_next_iff_trg_ex {cd : ChaseDerivation obs rules} : cd.next.isSome
     cases i with
     | zero =>
       apply not_active
-      have eq : cd.head = node := by simp only [ChaseDerivationSkeleton.head]; simp only [PossiblyInfiniteList.drop_zero, Option.mem_def] at node_mem; simp [node_mem]
+      have eq : cd.head = node := by unfold ChaseDerivationSkeleton.head; rw [Option.mem_def] at node_mem; grind
       rw [← eq]
       exact active
     | succ i =>
       simp only [ChaseDerivationSkeleton.next, ← PossiblyInfiniteList.empty_iff_head_none] at eq_none
-      rw [PossiblyInfiniteList.head_drop, ← PossiblyInfiniteList.get?_tail, eq_none, PossiblyInfiniteList.get?_empty] at node_mem
+      rw [PossiblyInfiniteList.head_drop, ← PossiblyInfiniteList.get?_tail, eq_none] at node_mem
       simp at node_mem
 
 end Next
@@ -160,7 +166,9 @@ def IsSuffix (cd1 cd2 : ChaseDerivation obs rules) : Prop := ChaseDerivationSkel
 infixl:50 " <:+ " => IsSuffix
 
 /-- Members of our suffix are also our members. -/
-theorem mem_of_mem_suffix {cd1 cd2 : ChaseDerivation obs rules} (suffix : cd1 <:+ cd2) : ∀ node ∈ cd1, node ∈ cd2 := ChaseDerivationSkeleton.mem_of_mem_suffix suffix
+@[grind ->]
+theorem mem_of_mem_suffix {cd1 cd2 : ChaseDerivation obs rules} (suffix : cd1 <:+ cd2) : ∀ node ∈ cd1, node ∈ cd2 :=
+  ChaseDerivationSkeleton.mem_of_mem_suffix suffix
 
 /-- Each `ChaseNode` in the `ChaseDerivation` induces a subderivation. -/
 theorem subderivation_of_node_mem {cd : ChaseDerivation obs rules} {node : ChaseNode obs rules} (node_mem : node ∈ cd) :
@@ -169,7 +177,8 @@ theorem subderivation_of_node_mem {cd : ChaseDerivation obs rules} {node : Chase
   exists cd.derivation_for_skeleton cds2 suffix
 
 /-- Fairness can be stated as: For each trigger, there exists a subderivation such that the trigger is not active for all nodes in the subderivation. -/
-theorem fairness' {cd : ChaseDerivation obs rules} : ∀ (trg : RTrigger obs rules), ∃ (cd2 : ChaseDerivation obs rules), cd2 <:+ cd ∧ ∀ node ∈ cd2, ¬ trg.val.active node.facts := by
+theorem fairness' {cd : ChaseDerivation obs rules} :
+    ∀ (trg : RTrigger obs rules), ∃ (cd2 : ChaseDerivation obs rules), cd2 <:+ cd ∧ ∀ node ∈ cd2, ¬ trg.val.active node.facts := by
   intro trg
   rcases cd.fairness trg with ⟨n, ⟨node, node_mem, fairness_head⟩, fairness_tail⟩
   let cds2 := cd.derivation_for_branch_suffix (cd.branch.drop n) (cd.branch.IsSuffix_drop n) (by rw [node_mem]; simp)
@@ -178,16 +187,12 @@ theorem fairness' {cd : ChaseDerivation obs rules} : ∀ (trg : RTrigger obs rul
   constructor
   . exact cd.branch.IsSuffix_drop n
   . intro node2 node2_mem
+    rw [mem_iff] at node2_mem
     rcases node2_mem with ⟨m, node2_mem⟩
-    simp only [cd2, derivation_for_skeleton, cds2, ChaseDerivationSkeleton.derivation_for_branch_suffix, PossiblyInfiniteList.drop, InfiniteList.get_drop] at node2_mem
+    simp only [cd2, derivation_for_skeleton, cds2, ChaseDerivationSkeleton.derivation_for_branch_suffix] at node2_mem
     cases m with
-    | zero => simp only [PossiblyInfiniteList.head_drop, PossiblyInfiniteList.get?] at node_mem; rw [Nat.add_zero, node_mem, Option.some_inj] at node2_mem; rw [← node2_mem]; exact fairness_head
-    | succ m =>
-      specialize fairness_tail m
-      simp only [PossiblyInfiniteList.get?_tail, PossiblyInfiniteList.get?_drop] at fairness_tail
-      simp only [PossiblyInfiniteList.get?] at fairness_tail
-      specialize fairness_tail node2 node2_mem
-      exact fairness_tail
+    | zero => grind
+    | succ m => apply fairness_tail m; grind
 
 end Suffixes
 
@@ -197,20 +202,27 @@ section Tail
 ### Tail
 -/
 
+@[expose]
 def tail (cd : ChaseDerivation obs rules) (next_some : cd.next.isSome) : ChaseDerivation obs rules :=
   cd.derivation_for_skeleton (ChaseDerivationSkeleton.tail cd.toChaseDerivationSkeleton next_some) (cd.branch.IsSuffix_tail)
 
 /-- The `head` of the `tail` is `next`. -/
-theorem head_tail {cd : ChaseDerivation obs rules} {next_some : cd.next.isSome} : some (cd.tail next_some).head = cd.next := ChaseDerivationSkeleton.head_tail
+theorem head_tail {cd : ChaseDerivation obs rules} {next_some : cd.next.isSome} : some (cd.tail next_some).head = cd.next :=
+  ChaseDerivationSkeleton.head_tail
 
 /-- The `head` of the `tail` is `next`. -/
-theorem head_tail' {cd : ChaseDerivation obs rules} {next_some : cd.next.isSome} : (cd.tail next_some).head = cd.next.get next_some := ChaseDerivationSkeleton.head_tail'
+@[simp, grind =]
+theorem head_tail' {cd : ChaseDerivation obs rules} {next_some : cd.next.isSome} : (cd.tail next_some).head = cd.next.get next_some :=
+  ChaseDerivationSkeleton.head_tail'
 
 /-- `next` is a member of the `tail`. -/
-theorem next_mem_tail {cd : ChaseDerivation obs rules} {next_some : cd.next.isSome} : ∀ next ∈ cd.next, next ∈ cd.tail next_some := ChaseDerivationSkeleton.next_mem_tail
+@[grind ->]
+theorem next_mem_tail {cd : ChaseDerivation obs rules} {next_some : cd.next.isSome} : ∀ next ∈ cd.next, next ∈ cd.tail next_some :=
+  ChaseDerivationSkeleton.next_mem_tail
 
 /-- A node is a member if and only if it is either the head or it is a member of the tail. -/
-theorem mem_iff_eq_head_or_mem_tail {cd : ChaseDerivation obs rules} {node : ChaseNode obs rules} : node ∈ cd ↔ node = cd.head ∨ ∃ h, node ∈ cd.tail h := ChaseDerivationSkeleton.mem_iff_eq_head_or_mem_tail
+theorem mem_iff_eq_head_or_mem_tail {cd : ChaseDerivation obs rules} {node : ChaseNode obs rules} : node ∈ cd ↔ node = cd.head ∨ ∃ h, node ∈ cd.tail h :=
+  ChaseDerivationSkeleton.mem_iff_eq_head_or_mem_tail
 
 /-- A derivation is a suffix of another if and only if both are the same or the first is a suffix of the second's tail. -/
 theorem suffix_iff_eq_or_suffix_tail {cd1 cd2 : ChaseDerivation obs rules} : cd1 <:+ cd2 ↔ cd1 = cd2 ∨ ∃ h, cd1 <:+ cd2.tail h := by
@@ -261,7 +273,7 @@ end InductionPrinciple
 
 end Basics
 
-section FactMonotonicity
+public section FactMonotonicity
 
 /-!
 ## Subset Monotonicity of Facts in ChaseNodes
@@ -270,11 +282,13 @@ Compared to `ChaseDerivationSkeleton`, we get a couple of nice implications out 
 -/
 
 /-- Each member's facts contain the head facts. Note that this extends to arbitrary pairs of members since each member always induces a subderivation where it acts as the head. -/
+@[grind <-]
 theorem facts_node_subset_every_mem {cd : ChaseDerivation obs rules} : ∀ node ∈ cd, cd.head.facts ⊆ node.facts :=
   ChaseDerivationSkeleton.facts_node_subset_every_mem
 
 /-- A first implication of `facts_node_subset_every_mem` is that, considering one of our subderivations, each of our members either has all of its facts contained in the head of the subderivation or it is itself a member of the subderivation. -/
-theorem mem_suffix_of_mem {cd1 cd2 : ChaseDerivation obs rules} (suffix : cd1 <:+ cd2) : ∀ node ∈ cd2, node.facts ⊆ cd1.head.facts ∨ node ∈ cd1 := ChaseDerivationSkeleton.mem_suffix_of_mem suffix
+theorem mem_suffix_of_mem {cd1 cd2 : ChaseDerivation obs rules} (suffix : cd1 <:+ cd2) : ∀ node ∈ cd2, node.facts ⊆ cd1.head.facts ∨ node ∈ cd1 :=
+  ChaseDerivationSkeleton.mem_suffix_of_mem suffix
 
 /-- The `head` cannot occur in the `tail`. Otherwise, it would be introduced using a trigger but then this trigger is already obsolete since all the facts from `head` already occur in the very beginning. We use `ObsoletenessCondition.contains_trg_result_implies_cond` here. -/
 theorem head_not_mem_tail {cd : ChaseDerivation obs rules} : ∀ h, ¬ cd.head ∈ cd.tail h := by
@@ -289,6 +303,7 @@ theorem head_not_mem_tail {cd : ChaseDerivation obs rules} : ∀ h, ¬ cd.head �
   exact cd2.head_mem
 
 /-- By `head_not_mem_tail`, if we have a suffix but our head occurs in the suffix, then our suffix is equal to us. -/
+@[grind ->]
 theorem eq_of_suffix_of_head_mem {cd1 cd2 : ChaseDerivation obs rules} (suffix : cd1 <:+ cd2) (head_mem : cd2.head ∈ cd1) : cd1 = cd2 := by
   rw [suffix_iff_eq_or_suffix_tail] at suffix
   cases suffix with
@@ -296,6 +311,7 @@ theorem eq_of_suffix_of_head_mem {cd1 cd2 : ChaseDerivation obs rules} (suffix :
   | inr suffix => rcases suffix with ⟨h, suffix⟩; apply False.elim; apply head_not_mem_tail h; apply mem_of_mem_suffix suffix; exact head_mem
 
 /-- And now by `eq_of_suffix_of_head_mem`, if we have two suffixes $C$ and $D$, and the head of $D$ occurs in $C$, then $D$ is a suffix of $C$. This may seem obvious even without the above results but it is really not even though it aligns well with one's intuition. Imagine that a `ChaseNode` could occur multiple times in a `ChaseDerivation`. Then we may have a case where $C$ is a subderivation of $D$, $D$ is not a subderivation of $C$ but $D$ occurs in $C$. -/
+@[grind ->]
 theorem suffix_of_suffix_of_suffix_of_head_mem {cd cd1 cd2 : ChaseDerivation obs rules} : cd1 <:+ cd -> cd2 <:+ cd -> cd2.head ∈ cd1 -> cd2 <:+ cd1 := by
   intro suffix1 suffix2 head_mem
   cases PossiblyInfiniteList.suffix_or_suffix_of_suffix suffix1 suffix2 with
@@ -304,7 +320,7 @@ theorem suffix_of_suffix_of_suffix_of_head_mem {cd cd1 cd2 : ChaseDerivation obs
 
 end FactMonotonicity
 
-section Predecessors
+public section Predecessors
 
 /-!
 ## Predecessor Relation
@@ -321,24 +337,14 @@ theorem predecessor_iff {cd : ChaseDerivation obs rules} (n1 n2 : Node cd) : n1 
   . rintro ⟨cd2, suf, head, mem⟩; exists cd2.toChaseDerivationSkeleton
 
 /-- The predecessor relation is antisymmetric. -/
+@[grind ->]
 theorem predecessor_antisymm {cd : ChaseDerivation obs rules} {n1 n2 : Node cd} : n1 ≼ n2 -> n2 ≼ n1 -> n1 = n2 := by
-  rw [predecessor_iff, predecessor_iff]
-  rintro ⟨cd1, suffix1, head_eq1, prec1⟩ ⟨cd2, suffix2, head_eq2, prec2⟩
-  have : cd1 = cd2 := by
-    apply eq_of_suffix_of_head_mem _ (by rw [head_eq2]; exact prec1)
-    apply suffix_of_suffix_of_suffix_of_head_mem suffix2 suffix1
-    rw [head_eq1]; exact prec2
-  apply Subtype.ext
-  rw [← head_eq1, ← head_eq2, this]
+  simp only [predecessor_iff]; grind
 
 /-- The predecessor relation is transitive. -/
+@[grind ->]
 theorem predecessor_trans {cd : ChaseDerivation obs rules} {n1 n2 n3 : Node cd} : n1 ≼ n2 -> n2 ≼ n3 -> n1 ≼ n3 := by
-  rw [predecessor_iff, predecessor_iff, predecessor_iff]
-  rintro ⟨cd1, suffix1, head_eq1, prec1⟩ ⟨cd2, suffix2, head_eq2, prec2⟩
-  exists cd1; simp only [suffix1, head_eq1, true_and]
-  apply mem_of_mem_suffix _ _ prec2
-  apply suffix_of_suffix_of_suffix_of_head_mem suffix1 suffix2
-  rw [head_eq2]; exact prec1
+  simp only [predecessor_iff]; grind
 
 /-- We can express fairness in terms of the predecessor relation: For each trigger, there is a node such that the trigger is not active for each of the node's successors. -/
 theorem fairness_prec {cd : ChaseDerivation obs rules} : ∀ (trg : RTrigger obs rules), ∃ (node : cd.Node), ∀ node2, node ≼ node2 -> ¬ trg.val.active node2.val.facts := by
@@ -351,6 +357,7 @@ theorem fairness_prec {cd : ChaseDerivation obs rules} : ∀ (trg : RTrigger obs
   rcases prec with ⟨cd3, suf3, head3, node2_mem_cd3⟩
   simp only at head3
   have : cd3 = cd2 := by
+    have : cd2.head ∈ cd2 := cd2.head_mem
     apply eq_of_suffix_of_head_mem _ (by rw [← head3]; exact cd3.head_mem)
     apply suffix_of_suffix_of_suffix_of_head_mem suffix suf3
     rw [head3]; exact cd2.head_mem
@@ -364,18 +371,17 @@ The strict version of the predecessor is a strict total order on `ChaseDerivatio
 -/
 
 /-- The strict predecessor relation is asymmetric. -/
+@[grind ->]
 theorem strict_predecessor_asymmetric {cd : ChaseDerivation obs rules} {n1 n2 : Node cd} : n1 ≺ n2 -> ¬ n2 ≺ n1 := by
   intro prec contra; apply prec.right; apply predecessor_antisymm prec.left contra.left
 
 /-- The strict predecessor relation is transitive. -/
+@[grind ->]
 theorem strict_predecessor_trans {cd : ChaseDerivation obs rules} {n1 n2 n3 : Node cd} : n1 ≺ n2 -> n2 ≺ n3 -> n1 ≺ n3 := by
   intro prec1 prec2
   constructor
-  . apply predecessor_trans prec1.left prec2.left
-  . intro contra
-    apply strict_predecessor_asymmetric prec1
-    rw [contra]
-    exact prec2
+  . exact predecessor_trans prec1.left prec2.left
+  . grind
 
 /-- The `head` is a strict predecessor of `next`. -/
 theorem head_strict_prec_next {cd : ChaseDerivation obs rules} : ∀ {next}, (mem : next ∈ cd.next) -> ⟨cd.head, cd.head_mem⟩ ≺ ⟨next, cd.next_mem_of_mem _ mem⟩ := by
@@ -384,19 +390,17 @@ theorem head_strict_prec_next {cd : ChaseDerivation obs rules} : ∀ {next}, (me
   . exact cd.head_prec_next next_mem
   . intro contra
     apply cd.head_not_mem_tail (by rw [next_mem]; simp)
-    rw [Subtype.mk.injEq] at contra
-    rw [contra]
-    apply cd.next_mem_tail
-    exact next_mem
+    grind
 
 /-- The facts of a strict successor cannot be a subset of our facts. This is because strict successor nodes can only be introduced by active triggers. But if a trigger only produces facts that already exist, then it cannot be active. -/
+@[grind ->]
 theorem facts_not_subset_of_strict_predecessor {cd : ChaseDerivation obs rules} {n1 n2 : Node cd} : n1 ≺ n2 -> ¬ n2.val.facts ⊆ n1.val.facts := by
   intro prec contra
   rcases (predecessor_iff _ _).mp prec.left with ⟨d, suf, head, mem⟩
   rcases cd.subderivation_of_node_mem n2.property with ⟨d2, head2, suf2⟩
   have suf3 : d2 <:+ d := suffix_of_suffix_of_suffix_of_head_mem suf suf2 (by rw [head2]; exact mem)
   cases ChaseDerivation.suffix_iff_eq_or_suffix_tail.mp suf3 with
-  | inl suf3 => apply prec.right; rw [Subtype.mk.injEq]; rw [← head2, suf3]; exact Eq.symm head
+  | inl suf3 => grind
   | inr suf3 =>
     rcases suf3 with ⟨next_some, suf3⟩
     rw [Option.isSome_iff_exists] at next_some
@@ -412,16 +416,14 @@ theorem facts_not_subset_of_strict_predecessor {cd : ChaseDerivation obs rules} 
         constructor
         . simp [d.head_tail', next_some]
         . apply ChaseDerivation.mem_of_mem_suffix suf3; rw [← head2]; exact d2.head_mem
-      rw [head]
-      apply Set.subset_trans (d.facts_node_subset_of_prec this)
-      exact contra
+      grind
     exact Set.subset_trans (by rw [d.facts_next next_some]; apply Set.subset_union_of_subset_right; apply Set.subset_refl) this
 
 end StrictPredecessor
 
 end Predecessors
 
-section ChaseResult
+public section ChaseResult
 
 /-!
 ## Chase Result
@@ -430,6 +432,7 @@ Compared to the `ChaseDerivationSkeleton`, the result is now a model for all rul
 -/
 
 /-- The result is a model of all rules. This is true because otherwise, there would be an active trigger on the result. But then, this trigger needs to be active for some node and the hence it needs to become inactive at some point due to fairness. Hence it cannot be active on the result. Contradiction! -/
+@[grind <-]
 theorem result_models_rules {cd : ChaseDerivation obs rules} : cd.result.modelsRules rules := by
   intro r r_mem subs subs_loaded
   let trg : Trigger obs := ⟨r, subs⟩
@@ -457,7 +460,7 @@ theorem result_models_rules {cd : ChaseDerivation obs rules} : cd.result.modelsR
 
 end ChaseResult
 
-section TermsInChase
+public section TermsInChase
 
 /-!
 ## Terms in the Chase
@@ -501,12 +504,9 @@ theorem constants_node_subset_constants_fs_union_constants_rules {cd : ChaseDeri
           rcases FunctionFreeConjunction.mem_vars.mp (origin.fst.val.rule.frontier_subset_vars_body v_mem) with ⟨a, a_mem, v_mem'⟩
           exists origin.fst.val.subs.apply_function_free_atom a
           constructor
-          . have := cd2.active_trigger_origin_next next_eq
-            apply this.left
+          . apply (cd2.active_trigger_origin_next next_eq).left
             rw [List.mem_toSet]
-            unfold PreTrigger.mapped_body
-            unfold GroundSubstitution.apply_function_free_conj
-            apply List.mem_map_of_mem
+            apply TermMapping.apply_generalized_atom_mem_apply_generalized_atom_list
             exact a_mem
           . unfold Fact.constants
             rw [List.mem_flatMap]
@@ -519,9 +519,8 @@ theorem constants_node_subset_constants_fs_union_constants_rules {cd : ChaseDeri
               constructor
               . exact v_mem'
               . unfold PreTrigger.subs_for_mapped_head at t_mem
-                rw [PreTrigger.apply_to_var_or_const_frontier_var] at t_mem
-                . exact t_mem
-                . exact v_mem
+                rw [PreTrigger.apply_to_var_or_const_frontier_var _ _ _ v_mem] at t_mem
+                exact t_mem
             . exact c_mem
         | inr c_mem =>
           apply Or.inr
@@ -529,11 +528,7 @@ theorem constants_node_subset_constants_fs_union_constants_rules {cd : ChaseDeri
           constructor
           . exact origin.fst.property
           . unfold Rule.head_constants
-            rw [List.mem_flatMap]
-            exists origin.fst.val.rule.head[origin.snd.val]'(by rw [← PreTrigger.length_mapped_head]; exact origin.snd.isLt)
-            constructor
-            . apply List.get_mem
-            . exact c_mem
+            grind
       . exact c_mem
 
 /-- Each functional term in the chase originates as a fresh term from a trigger if it was not already part of the initial fact set. -/
@@ -566,7 +561,7 @@ theorem functional_term_originates_from_some_trigger
       unfold ChaseNode.origin_result at t_mem
       rw [FactSet.mem_terms_toSet, PreTrigger.mem_terms_mapped_head_iff] at t_mem
       cases t_mem with
-      | inl t_mem => rcases t_is_func with ⟨func, ts, arity, t_is_func⟩; rcases t_mem with ⟨c, _, t_mem⟩; rw [← t_mem] at t_is_func; simp [GroundTerm.const, GroundTerm.func] at t_is_func
+      | inl t_mem => rcases t_is_func with ⟨func, ts, arity, t_is_func⟩; rcases t_mem with ⟨c, _, t_mem⟩; rw [← t_mem] at t_is_func; apply False.elim; exact GroundTerm.func_neq_const (Eq.symm t_is_func)
       | inr t_mem =>
       cases t_mem with
       | inr t_mem =>
@@ -600,7 +595,7 @@ theorem trigger_introducing_functional_term_occurs_in_chase
     cases eq : t with
     | const _ =>
       rw [eq] at t_mem_trg
-      simp [PreTrigger.fresh_terms_for_head_disjunct, PreTrigger.functional_term_for_var, GroundTerm.func, GroundTerm.const] at t_mem_trg
+      simp [PreTrigger.fresh_terms_for_head_disjunct, PreTrigger.functional_term_for_var, GroundTerm.func_neq_const] at t_mem_trg
     | func func ts arity_ok => exists func, ts, arity_ok
   ) t_mem_node with
   | inl t_mem => apply Or.inl; exact t_mem
@@ -647,7 +642,7 @@ theorem node_has_unique_position (cd : ChaseDerivation obs rules) : ∀ node, �
   intro node i j lt eq_i eq_j
   have le := Nat.le_pred_of_lt lt
   let cds2 := cd.derivation_for_branch_suffix (cd.branch.drop j.pred) (PossiblyInfiniteList.IsSuffix_drop j.pred) (by
-    rw [Option.isSome_iff_ne_none]; intro contra
+    rw [Option.isSome_iff_ne_none, PossiblyInfiniteList.head_drop]; intro contra
     have := cd.branch.no_holes' j.pred contra
     rw [Nat.succ_pred (Nat.ne_zero_of_lt lt)] at this
     rw [eq_j] at this
@@ -669,10 +664,10 @@ theorem node_has_unique_position (cd : ChaseDerivation obs rules) : ∀ node, �
       constructor; exact PossiblyInfiniteList.IsSuffix_drop i
       constructor; simp [eq_i, node]
       apply ChaseDerivationSkeleton.mem_of_mem_suffix (cd1 := cds2) _ _ cd2.head_mem
+      rw [ChaseDerivationSkeleton.IsSuffix_iff]
       exists j.pred - i
-      simp only [cds2, ChaseDerivationSkeleton.derivation_for_branch_suffix, PossiblyInfiniteList.drop]
-      apply InfiniteList.ext; intro n
-      simp only [InfiniteList.get_drop, ← Nat.add_assoc, Nat.add_sub_of_le le]
+      simp only [cds2, ChaseDerivationSkeleton.derivation_for_branch_suffix]
+      grind
     exact cd.facts_node_subset_of_prec prec
   exact Set.subset_trans (node.facts_contain_origin_result (node.origin.get (cd2.isSome_origin_next next_eq)) (by simp)) sub
 
@@ -684,7 +679,7 @@ theorem get?_branch_injective (cd : ChaseDerivation obs rules) : ∀ node, ∀ i
   | inl lt => exact cd.node_has_unique_position node i j lt eq_i eq_j
   | inr lt => exact cd.node_has_unique_position node j i lt eq_j eq_i
 
-theorem prop_for_node_has_minimal_such_node {cd : ChaseDerivation obs rules} (prop : cd.Node -> Prop) :
+public theorem prop_for_node_has_minimal_such_node {cd : ChaseDerivation obs rules} (prop : cd.Node -> Prop) :
     ∀ n, prop n -> ∃ n2, prop n2 ∧ ∀ n3, n3 ≺ n2 -> ¬ prop n3 := by
   let prop' : Nat -> Prop := fun i => ∃ (e : ChaseNode obs rules) (mem : e ∈ cd.branch.get? i), prop ⟨e, by exists i⟩
   intro n prop_n
@@ -703,16 +698,17 @@ theorem prop_for_node_has_minimal_such_node {cd : ChaseDerivation obs rules} (pr
       have n2_mem' : n2 ∈ cd := by exists k
       rcases cd.subderivation_of_node_mem n2_mem' with ⟨cd2, head2, suf2⟩
       exists cd2; simp only [suf2, head2, true_and]
+      rw [mem_iff]
       exists j - k
-      rcases suf2 with ⟨k', suf2⟩
+      unfold IsSuffix at suf2; rw [ChaseDerivationSkeleton.IsSuffix_iff] at suf2; rcases suf2 with ⟨k', suf2⟩
       have : k' = k := by
         apply cd.get?_branch_injective n2
         . rw [← head2]
-          simp only [ChaseDerivationSkeleton.head, Option.some_get, PossiblyInfiniteList.head]
+          simp only [ChaseDerivationSkeleton.head, Option.some_get]
           rw [← suf2]
-          rfl
+          simp
         . exact n2_mem
-      rw [← suf2, this, InfiniteList.get_drop, Nat.add_sub_of_le le]
+      rw [← suf2, this, PossiblyInfiniteList.get?_drop, Nat.add_sub_of_le le]
       exact n3_mem
     . exact Ne.symm prec.right⟩
   exists n3.val, n3_mem
