ExistentialRules/ChaseSequence/ChaseDerivationSkeleton.lean
@@ -1,6 +1,8 @@
-import PossiblyInfiniteTrees.PossiblyInfiniteList.PossiblyInfiniteList
+module
 
-import ExistentialRules.ChaseSequence.ChaseNode
+public import PossiblyInfiniteTrees.PossiblyInfiniteList.PossiblyInfiniteList
+
+public import ExistentialRules.ChaseSequence.ChaseNode
 
 /-!
 # Chase Derivation Skeleton
@@ -12,6 +14,8 @@ We only demand a `PossiblyInfiniteList` of `ChaseNode`s that is non-empty such t
 We also do not care here whether the derivation is "fair".
 -/
 
+public section
+
 variable {sig : Signature} [DecidableEq sig.P] [DecidableEq sig.C] [DecidableEq sig.V]
 
 section ChaseStep
@@ -22,6 +26,7 @@ section ChaseStep
 To define how one chase step follows from the previous, we introduce an auxiliary definitions that capture that the next `ChaseNode` in a `ChaseDerivationSkeleton` always follows from the previous from a trigger application, given that a next node still exists.
 -/
 
+@[expose]
 def exists_trigger_opt_fs (obs : ObsoletenessCondition sig) (rules : RuleSet sig) (before : ChaseNode obs rules) (after : Option (ChaseNode obs rules)) : Prop :=
   ∀ node ∈ after,
   ∃ trg : (RTrigger (obs : LaxObsoletenessCondition sig) rules),
@@ -66,7 +71,11 @@ Here we introduce some auxiliary definitions and theorems and we lift some of th
 instance : Membership (ChaseNode obs rules) (ChaseDerivationSkeleton obs rules) where
   mem cd node := node ∈ cd.branch
 
+/-- An element is a member of the derivation iff it occurs at some index in the underlying branch. -/
+theorem mem_iff {cd : ChaseDerivationSkeleton obs rules} : ∀ {e}, e ∈ cd ↔ ∃ n, cd.branch.get? n = some e := by rfl
+
 /-- Each suffix of the underlying `PossiblyInfiniteList` is itself a `ChaseDerivationSkeleton` as long as its head is not none. -/
+@[expose]
 def derivation_for_branch_suffix
     (cd : ChaseDerivationSkeleton obs rules)
     (l2 : PossiblyInfiniteList (ChaseNode obs rules))
@@ -81,13 +90,15 @@ def derivation_for_branch_suffix
     rw [← suffix]
     intro n
     have := cd.triggers_exist (m + n)
-    simp only [PossiblyInfiniteList.head_drop, PossiblyInfiniteList.get?_drop] at *
+    simp only [PossiblyInfiniteList.head_drop, PossiblyInfiniteList.get?_drop, PossiblyInfiniteList.tail_drop] at *
     exact this
 
 /-- The head of the `ChaseDerivationSkeleton` is the initial `ChaseNode`. We know that this is never none. -/
+@[expose]
 def head (cd : ChaseDerivationSkeleton obs rules) : ChaseNode obs rules := cd.branch.head.get (cd.isSome_head)
 
 /-- The `head` is a member. -/
+@[grind <-]
 theorem head_mem {cd : ChaseDerivationSkeleton obs rules} : cd.head ∈ cd := by exists 0; simp [head, PossiblyInfiniteList.head_eq, PossiblyInfiniteList.get?]
 
 section Next
@@ -99,12 +110,16 @@ For a `ChaseDerivationSkeleton` derivation, its `next` node is the `ChaseNode` i
 We mainly introduce a couple of theorems here that abstract away the `triggers_exist` condition from the `ChaseDerivationSkeleton` definition.
 -/
 
+@[expose]
 def next (cd : ChaseDerivationSkeleton obs rules) : Option (ChaseNode obs rules) := cd.branch.tail.head
 
 /-- The `next` node is a member. -/
-theorem next_mem_of_mem {cd : ChaseDerivationSkeleton obs rules} : ∀ next ∈ cd.next, next ∈ cd := by intro next next_mem; apply cd.branch.tail.mem_of_mem_suffix cd.branch.IsSuffix_tail; apply cd.branch.tail.head_mem; exact next_mem
+@[grind ->]
+theorem next_mem_of_mem {cd : ChaseDerivationSkeleton obs rules} : ∀ next ∈ cd.next, next ∈ cd := by
+  intro next next_mem; apply cd.branch.tail.mem_of_mem_suffix cd.branch.IsSuffix_tail; apply cd.branch.tail.head_mem; exact next_mem
 
 /-- The origin of the `next` `ChaseNode` needs to be set. -/
+@[grind ->]
 theorem isSome_origin_next {cd : ChaseDerivationSkeleton obs rules} {next : ChaseNode obs rules} (eq : cd.next = some next) : next.origin.isSome := by
   have trg_ex := cd.triggers_exist 0 cd.head (by simp [PossiblyInfiniteList.drop_zero, head])
   rw [PossiblyInfiniteList.drop_zero] at trg_ex
@@ -129,24 +144,32 @@ section Suffixes
 We define a suffix relation on `ChaseDerivationSkeleton` simply as the suffix relation of the underlying `PossiblyInfiniteList`.
 -/
 
+@[expose]
 def IsSuffix (cd1 cd2 : ChaseDerivationSkeleton obs rules) : Prop := cd1.branch <:+ cd2.branch
 infixl:50 " <:+ " => IsSuffix
 
+/-- Unfolds the definition of the suffix relation. -/
+theorem IsSuffix_iff {cd1 cd2 : ChaseDerivationSkeleton obs rules} : cd1 <:+ cd2 ↔ ∃ m, cd2.branch.drop m = cd1.branch := PossiblyInfiniteList.IsSuffix_iff
+
 /-- Members of our suffix are also our members. -/
+@[grind ->]
 theorem mem_of_mem_suffix {cd1 cd2 : ChaseDerivationSkeleton obs rules} (suffix : cd1 <:+ cd2) : ∀ node ∈ cd1, node ∈ cd2 := by
-  rintro node ⟨n, node_eq⟩
+  simp only [mem_iff]
+  intro node ⟨n, node_eq⟩
+  rw [IsSuffix_iff] at suffix
   rcases suffix with ⟨m, suffix⟩
   exists m + n
-  rw [← suffix, InfiniteList.get_drop] at node_eq
+  rw [← suffix, PossiblyInfiniteList.get?_drop] at node_eq
   exact node_eq
 
 /-- Each `ChaseNode` in the `ChaseDerivationSkeleton` induces a subderivation. -/
 theorem subderivation_of_node_mem {cd : ChaseDerivationSkeleton obs rules} {node : ChaseNode obs rules} (node_mem : node ∈ cd) :
     ∃ (cd2 : ChaseDerivationSkeleton obs rules), cd2.head = node ∧ cd2 <:+ cd := by
+  rw [mem_iff] at node_mem
   rcases node_mem with ⟨n, node_mem⟩
-  exists cd.derivation_for_branch_suffix (cd.branch.drop n) (cd.branch.IsSuffix_drop n) (by simp only [PossiblyInfiniteList.head_drop, PossiblyInfiniteList.get?, node_mem]; simp)
+  exists cd.derivation_for_branch_suffix (cd.branch.drop n) (cd.branch.IsSuffix_drop n) (by simp [node_mem])
   constructor
-  . simp only [derivation_for_branch_suffix, head, PossiblyInfiniteList.head_drop, PossiblyInfiniteList.get?, node_mem, Option.get_some]
+  . simp [derivation_for_branch_suffix, head, node_mem]
   . exact cd.branch.IsSuffix_drop n
 
 end Suffixes
@@ -159,6 +182,7 @@ section Tail
 If `next` exists, we can drop the first element from the `ChaseDerivationSkeleton` and obtain a new `ChaseDerivationSkeleton`, which, inspired by the `PossiblyInfiniteList`, we call the `tail`.
 -/
 
+@[expose]
 def tail (cd : ChaseDerivationSkeleton obs rules) (next_some : cd.next.isSome) : ChaseDerivationSkeleton obs rules :=
   cd.derivation_for_branch_suffix cd.branch.tail (cd.branch.IsSuffix_tail) next_some
 
@@ -168,9 +192,11 @@ theorem head_tail {cd : ChaseDerivationSkeleton obs rules} {next_some : cd.next.
   simp only [Option.some_get]
 
 /-- The `head` of the `tail` is `next`. -/
+@[simp, grind =]
 theorem head_tail' {cd : ChaseDerivationSkeleton obs rules} {next_some : cd.next.isSome} : (cd.tail next_some).head = cd.next.get next_some := by rfl
 
 /-- `next` is a member of the `tail`. -/
+@[grind ->]
 theorem next_mem_tail {cd : ChaseDerivationSkeleton obs rules} {next_some : cd.next.isSome} : ∀ next ∈ cd.next, next ∈ cd.tail next_some := by
   intro next next_mem
   have : next = cd.next.get next_some := by
@@ -180,55 +206,53 @@ theorem next_mem_tail {cd : ChaseDerivationSkeleton obs rules} {next_some : cd.n
   exact head_mem
 
 /-- A node is a member if and only if it is either the head or it is a member of the tail. -/
-theorem mem_iff_eq_head_or_mem_tail {cd : ChaseDerivationSkeleton obs rules} {node : ChaseNode obs rules} : node ∈ cd ↔ node = cd.head ∨ ∃ h, node ∈ cd.tail h := by
+theorem mem_iff_eq_head_or_mem_tail {cd : ChaseDerivationSkeleton obs rules} {node : ChaseNode obs rules} :
+    node ∈ cd ↔ node = cd.head ∨ ∃ h, node ∈ cd.tail h := by
   constructor
-  . rintro ⟨n, mem⟩
+  . rw [mem_iff]
+    intro ⟨n, mem⟩
     cases n with
-    | zero => apply Or.inl; simp [head, PossiblyInfiniteList.head, InfiniteList.head, mem]
+    | zero => apply Or.inl; simp [head, PossiblyInfiniteList.head_eq, mem]
     | succ n =>
-      apply Or.inr;
+      apply Or.inr
       exists (by
         rw [Option.isSome_iff_ne_none]; intro contra; simp only [next, PossiblyInfiniteList.head_eq, PossiblyInfiniteList.get?_tail] at contra
-        have := cd.branch.get?_eq_none_of_le_of_eq_none contra n.succ (by simp)
-        simp only [PossiblyInfiniteList.get?] at this; rw [this] at mem
+        rw [cd.branch.get?_eq_none_of_le_of_eq_none contra n.succ (by simp)] at mem
         simp at mem)
+      rw [mem_iff]
       exists n
+      simpa [tail, derivation_for_branch_suffix] using mem
   . intro or; cases or with
     | inl eq_head => rw [eq_head]; exact cd.head_mem
     | inr mem_tail => rcases mem_tail with ⟨_, mem_tail⟩; apply mem_of_mem_suffix _ _ mem_tail; exact cd.branch.IsSuffix_tail
 
 /-- A derivation is a suffix of another if and only if both are the same or the first is a suffix of the second's tail. -/
 theorem suffix_iff_eq_or_suffix_tail {cd1 cd2 : ChaseDerivationSkeleton obs rules} : cd1 <:+ cd2 ↔ cd1 = cd2 ∨ ∃ h, cd1 <:+ cd2.tail h := by
-  -- TODO: maybe we should extract a result like this to InfiniteList directly
+  -- TODO: maybe we should extract a result like this to (Possibly)InfiniteList directly
   constructor
-  . rintro ⟨n, suffix⟩
+  . rw [IsSuffix_iff]
+    intro ⟨n, suffix⟩
     cases n with
-    | zero => apply Or.inl; rw [InfiniteList.drop_zero] at suffix; apply Eq.symm; rw [ChaseDerivationSkeleton.mk.injEq, PossiblyInfiniteList.mk.injEq]; exact suffix
+    | zero => apply Or.inl; rw [PossiblyInfiniteList.drop_zero] at suffix; apply Eq.symm; rw [ChaseDerivationSkeleton.mk.injEq]; exact suffix
     | succ n =>
       apply Or.inr
       exists (by
         rw [Option.isSome_iff_ne_none]
         intro contra
+        simp only [next, PossiblyInfiniteList.head_eq, PossiblyInfiniteList.get?_tail] at contra
         have := cd2.branch.get?_eq_none_of_le_of_eq_none contra (n+1) (by simp)
-        simp only [PossiblyInfiniteList.get?] at this
-        rw [InfiniteList.ext_iff] at suffix
+        rw [PossiblyInfiniteList.ext_iff] at suffix
         specialize suffix 0
-        rw [InfiniteList.get_drop, Nat.add_zero, this] at suffix
+        rw [PossiblyInfiniteList.get?_drop, Nat.add_zero, this] at suffix
         have contra := cd1.isSome_head
         rw [Option.isSome_iff_ne_none] at contra
         apply contra
-        simp only [PossiblyInfiniteList.head_eq, PossiblyInfiniteList.get?]
+        simp only [PossiblyInfiniteList.head_eq]
         rw [← suffix])
+      rw [IsSuffix_iff]
       exists n
-      simp only [tail, derivation_for_branch_suffix, PossiblyInfiniteList.tail]
-      apply InfiniteList.ext
-      intro m
-      simp only [InfiniteList.get_tail, InfiniteList.get_drop]
-      rw [InfiniteList.ext_iff] at suffix
-      simp only [InfiniteList.get_drop] at suffix
-      have : (n+m).succ = (n + 1 + m) := by omega
-      rw [this]
-      apply suffix m
+      simp only [tail, derivation_for_branch_suffix]
+      grind
   . intro h; cases h with
     | inl eq => rw [eq]; exact PossiblyInfiniteList.IsSuffix_refl
     | inr suffix => rcases suffix with ⟨h, suffix⟩; apply PossiblyInfiniteList.IsSuffix_trans suffix; exact PossiblyInfiniteList.IsSuffix_tail
@@ -248,7 +272,9 @@ For this, we introduce `ChaseDerivationSkeleton.Node` as the subtype of `ChaseNo
 abbrev Node (cd : ChaseDerivationSkeleton obs rules) := { node : ChaseNode obs rules // node ∈ cd}
 
 /-- A `Node` of our suffix can be cast into our `Node` type. -/
-def Node.cast_suffix {cd cd2 : ChaseDerivationSkeleton obs rules} (suffix : cd <:+ cd2) (node : Node cd) : Node cd2 := ⟨node.val, mem_of_mem_suffix suffix _ node.property⟩
+@[expose]
+def Node.cast_suffix {cd cd2 : ChaseDerivationSkeleton obs rules} (suffix : cd <:+ cd2) (node : Node cd) : Node cd2 :=
+  ⟨node.val, mem_of_mem_suffix suffix _ node.property⟩
 
 /-- If we want to show a motive for all nodes in a derivation, it is enough to show the motive for the head and for the next node in each abitrary subderivation where the motive already holds for the head. This can be used with the induction tactic. -/
 theorem mem_rec
@@ -283,18 +309,15 @@ theorem mem_tail_iff {cd : ChaseDerivationSkeleton obs rules} {next_some : cd.ne
       exists cd3; constructor
       . apply cd3.branch.IsSuffix_trans suffix; exact cd.branch.IsSuffix_tail
       . exact next_mem
-  . rintro ⟨cd2, suffix, next_eq⟩
+  . intro ⟨cd2, suffix, next_eq⟩
     have : cd2.tail (by simp [next_eq]) <:+ cd.tail next_some := by
-      -- TODO: maybe we should extract a result like this to InfiniteList directly
+      -- TODO: maybe we should extract a result like this to (Possibly)InfiniteList directly
+      rw [IsSuffix_iff] at suffix
       rcases suffix with ⟨n, suffix⟩
+      rw [IsSuffix_iff]
       exists n
-      simp only [tail, derivation_for_branch_suffix, PossiblyInfiniteList.tail]
-      apply InfiniteList.ext
-      intro m
-      simp only [InfiniteList.get_tail, InfiniteList.get_drop]
-      rw [InfiniteList.ext_iff] at suffix
-      simp only [InfiniteList.get_drop] at suffix
-      apply suffix m.succ
+      simp only [tail, derivation_for_branch_suffix]
+      grind
     apply mem_of_mem_suffix this
     rw [← head_tail (next_some := by simp [next_eq]), Option.some_inj] at next_eq
     simp only [← next_eq]
@@ -313,6 +336,7 @@ Since `ChaseNodes` always extend the previous facts, the fact sets can only be g
 -/
 
 /-- Each member's facts contain the head facts. Note that this extends to arbitrary pairs of members since each member always induces a subderivation where it acts as the head. -/
+@[grind <-]
 theorem facts_node_subset_every_mem {cd : ChaseDerivationSkeleton obs rules} : ∀ node ∈ cd, cd.head.facts ⊆ node.facts := by
   intro node node_mem
   let node' : cd.Node := ⟨node, node_mem⟩
@@ -345,11 +369,14 @@ At this point, it does not have many properties. On Proper `ChaseDerivation`s it
 -/
 
 /-- A node $n$ is a predecessor of a node $m$ if there is a subderivation there $n$ is the head and $m$ is an arbitrary member. -/
+@[expose]
 def predecessor {cd : ChaseDerivationSkeleton obs rules} (n1 n2 : Node cd) : Prop := ∃ cd2, cd2 <:+ cd ∧ cd2.head = n1.val ∧ n2.val ∈ cd2
 infixl:50 " ≼ " => predecessor
 
 /-- The predecessor relation is stable across suffixes. That is, predecessor in our suffix are also predecessor for us. We only need to cast the nodes. -/
-theorem predecessor_of_suffix {cd cd2 : ChaseDerivationSkeleton obs rules} {n1 n2 : Node cd} (suffix : cd <:+ cd2) : n1 ≼ n2 -> (n1.cast_suffix suffix) ≼ (n2.cast_suffix suffix) := by
+@[grind <-]
+theorem predecessor_of_suffix {cd cd2 : ChaseDerivationSkeleton obs rules} {n1 n2 : Node cd} (suffix : cd <:+ cd2) :
+    n1 ≼ n2 -> (n1.cast_suffix suffix) ≼ (n2.cast_suffix suffix) := by
   rintro ⟨cd3, suffix', head_eq, mem⟩
   exists cd3; constructor
   . exact cd3.branch.IsSuffix_trans suffix' suffix
@@ -358,7 +385,9 @@ theorem predecessor_of_suffix {cd cd2 : ChaseDerivationSkeleton obs rules} {n1 n
   . exact mem
 
 /-- The predecessor relation is reflexive. -/
-theorem predecessor_refl {cd : ChaseDerivationSkeleton obs rules} {node : Node cd} : node ≼ node := by rcases cd.subderivation_of_node_mem node.property with ⟨cd2, head_eq, suffix⟩; exists cd2; simp only [suffix, head_eq, true_and]; rw [← head_eq]; exact cd2.head_mem
+@[grind <-]
+theorem predecessor_refl {cd : ChaseDerivationSkeleton obs rules} {node : Node cd} : node ≼ node := by
+  rcases cd.subderivation_of_node_mem node.property with ⟨cd2, head_eq, suffix⟩; exists cd2; simp only [suffix, head_eq, true_and]; rw [← head_eq]; exact cd2.head_mem
 
 /-- The predecessor relation is total. -/
 theorem predecessor_total {cd : ChaseDerivationSkeleton obs rules} (n1 n2 : Node cd) : n1 ≼ n2 ∨ n2 ≼ n1 := by
@@ -373,6 +402,7 @@ theorem head_prec_next {cd : ChaseDerivationSkeleton obs rules} : ∀ {next}, (m
   intro next next_mem; exact ⟨cd, cd.branch.IsSuffix_refl, rfl, cd.next_mem_of_mem _ next_mem⟩
 
 /-- The facts of our predecessor are a subset of our facts. -/
+@[grind ->]
 theorem facts_node_subset_of_prec {cd : ChaseDerivationSkeleton obs rules} {node1 node2 : cd.Node} : node1 ≼ node2 -> node1.val.facts ⊆ node2.val.facts := by
   rintro ⟨cd2, suffix, head_eq, mem⟩
   rw [← head_eq]
@@ -387,10 +417,12 @@ We also define a strict version of the predecessor relation (`≺`) in the obvio
 -/
 
 /-- A node is a strict predecessor of another if it is a predecessor but not equal. -/
+@[expose]
 def strict_predecessor {cd : ChaseDerivationSkeleton obs rules} (n1 n2 : Node cd) : Prop := n1 ≼ n2 ∧ n1 ≠ n2
 infixl:50 " ≺ " => strict_predecessor
 
 /-- As for the predecessor relation, we can show that the relation is stable across suffixes given that we cast the nodes. -/
+@[grind <-]
 theorem strict_predecessor_of_suffix {cd cd2 : ChaseDerivationSkeleton obs rules} {n1 n2 : Node cd} (suffix : cd <:+ cd2) : n1 ≺ n2 -> (n1.cast_suffix suffix) ≺ (n2.cast_suffix suffix) := by
   intro prec
   constructor
@@ -398,6 +430,7 @@ theorem strict_predecessor_of_suffix {cd cd2 : ChaseDerivationSkeleton obs rules
   . simp only [Node.cast_suffix]; intro contra; rw [Subtype.mk.injEq] at contra; apply prec.right; rw [Subtype.mk.injEq]; exact contra
 
 /-- The strict predecessor relation is irreflexive. -/
+@[grind <-]
 theorem strict_predecessor_irreflexive {cd : ChaseDerivationSkeleton obs rules} {n : Node cd} : ¬ n ≺ n := by intro contra; apply contra.right; rfl
 
 /-- The strict predecessor relation is total. -/
@@ -426,16 +459,18 @@ section ChaseResult
 Here, we define the result of a `ChaseDerivationSkeleton`, which is simply the `FactSet` that is the union of all facts of all `ChaseNode`s.
 -/
 
+@[expose]
 def result (cd : ChaseDerivationSkeleton obs rules) : FactSet sig :=
   fun f => ∃ node ∈ cd, f ∈ node.facts
 
 /-- Every node's facts occur in the result. -/
+@[grind <-]
 theorem facts_node_subset_result {cd : ChaseDerivationSkeleton obs rules} : ∀ node ∈ cd, node.facts ⊆ cd.result := by intro node _ _ _; exists node
 
 /-- The result of our suffix is the same our result. -/
+@[grind ->]
 theorem result_suffix {cd1 cd2 : ChaseDerivationSkeleton obs rules} (suffix : cd1 <:+ cd2) : cd1.result = cd2.result := by
-  apply Set.ext
-  intro f
+  ext f
   constructor
   . rintro ⟨node, node_mem, f_mem⟩; apply cd2.facts_node_subset_result; exact mem_of_mem_suffix suffix _ node_mem; exact f_mem
   . rintro ⟨node, node_mem, f_mem⟩
@@ -444,7 +479,8 @@ theorem result_suffix {cd1 cd2 : ChaseDerivationSkeleton obs rules} (suffix : cd
     | inr mem_suffix => apply cd1.facts_node_subset_result; exact mem_suffix; exact f_mem
 
 /-- For each (finite) list of facts in the result, there is a node that that contains all of them. -/
-theorem facts_mem_some_node_of_mem_result {cd : ChaseDerivationSkeleton obs rules} : ∀ (l : List (Fact sig)), l.toSet ⊆ cd.result -> ∃ node ∈ cd, l.toSet ⊆ node.facts := by
+theorem facts_mem_some_node_of_mem_result {cd : ChaseDerivationSkeleton obs rules} :
+    ∀ (l : List (Fact sig)), l.toSet ⊆ cd.result -> ∃ node ∈ cd, l.toSet ⊆ node.facts := by
   intro l
   induction l with
   | nil => intros; exists cd.head; constructor; exact cd.head_mem; intro _ contra; simp [List.mem_toSet] at contra
@@ -477,7 +513,8 @@ theorem facts_mem_some_node_of_mem_result {cd : ChaseDerivationSkeleton obs rule
           rw [cd_f_head]; exact f_mem
 
 /-- If a trigger is loaded for the result, then it is loaded for some node in the derivation. -/
-theorem trg_loaded_for_some_node_of_trg_loaded_for_result {cd : ChaseDerivationSkeleton obs rules} : ∀ trg : Trigger obs, trg.loaded cd.result -> ∃ node ∈ cd, trg.loaded node.facts := by
+theorem trg_loaded_for_some_node_of_trg_loaded_for_result {cd : ChaseDerivationSkeleton obs rules} :
+    ∀ trg : Trigger obs, trg.loaded cd.result -> ∃ node ∈ cd, trg.loaded node.facts := by
   intro trg trg_loaded
   apply cd.facts_mem_some_node_of_mem_result
   exact trg_loaded
